test/chain_trans.lean
@@ -12,7 +12,7 @@ begin
   have : w < w,
   { success_if_fail_with_msg
     { chain_trans }
-    "`w < w` cannot be proved from `w ≤ w`",
+    "no appropriate chain of inequalities can be found between `w` and `w`",
     admit },
   triv
 end
@@ -22,12 +22,17 @@ begin
   have : x < w,
   { success_if_fail_with_msg
     { chain_trans }
-    "no chain of inequalities can be found between `x` and `w`",
+    "no appropriate chain of inequalities can be found between `x` and `w`",
     admit },
   triv
 end
 
 example {w x y z : ℕ} {a b : ℤ} (h₀ : w ≤ x) (h₁ : x = y) (h₂ : y < z) : w < z :=
+begin
+  chain_trans,
+end
+
+example {w x y z : ℕ} {a b : ℤ} (h₀ : w ≤ x) (h₁ : x = y) (h₃ : y ≤ z) (h₂ : y < z) (h₃ : y ≤ z) : w < z :=
 begin
   chain_trans,
 end
